adding Zeta.Ghost

generic/Zeta.GenericVerifier.fst
@@ -1,16 +1,8 @@
 module Zeta.GenericVerifier
 
+open Zeta.Ghost
 open Zeta.SeqIdx
 open FStar.Classical
-
-let hoist_ghost #_ #_ _ = admit ()
-
-let hoist_ghost2 (#a:Type) (#b:a -> Type) (#c:(x:a -> b x -> Type)) (f:(x:a -> y:b x -> GTot (c x y))) = admit ()
-
-let hoist_ghost2_apply #_ #_ #_ _ _ _ = admit ()
-
-let hoist_ghost_restricted (#a:Type) (#b:a -> Type) (f:restricted_g_t a b)
-  : GTot (g:restricted_t a b{forall x. f x == g x}) = admit ()
 
 let not_contains_app_key (#vspec:_)
   (vtls: vspec.vtls_t{vspec.valid vtls})
